proof/JRussell/Basic.v
@@ -1,0 +1,77 @@
+Require Import Lambda.Terms.
+Require Import Lambda.LiftSubst.
+Require Import Lambda.Reduction.
+Require Import Lambda.Conv.
+Require Import Lambda.Env.
+Require Import JRussell.Types.
+
+Set Implicit Arguments.
+
+Implicit Types i k m n p : nat.
+Implicit Type s : sort.
+Implicit Types A B M N T t u v : term.
+
+Lemma lift_sort : forall n t s, lift n t = Srt s -> t = Srt s.
+Proof.
+  induction t ; simpl ; intros ; try discriminate.
+  simpl in H ; auto.
+Qed.
+
+Lemma left_not_kind : forall G t T, G |- t : T -> t <> Srt kind.
+Proof.
+  induction 1 ; intros ; unfold not ; intros ; try discriminate ; auto with coc.
+  apply IHtyp1.
+  pose (lift_sort 1 _ H1).
+  assumption.
+Qed.
+
+Lemma coerce_prop_prop : nil |- Srt prop >> Srt prop : kind.
+Proof.
+  intros.
+  auto with coc.
+Qed.
+
+Lemma coerce_set_set : nil |- Srt set >> Srt set : kind.
+Proof.
+  intros.
+  auto with coc.
+Qed.
+
+Lemma coerce_is_prop : forall s, is_prop s -> nil |- Srt s >> Srt s : kind.
+Proof.
+  intros.
+  induction H ;
+  rewrite H ; auto with coc.
+Qed.
+
+Lemma consistency_ind :
+  (forall e t T, e |- t : T -> consistent e) /\
+  (forall e T U s, e |- T >> U : s -> consistent e) /\
+  (forall e U V T, e |- U = V : T -> consistent e).
+Proof.
+  apply typ_coerce_jeq_ind with
+  (P:=fun e t T => fun H: e |- t : T => consistent e)
+  (P1 := fun e U V T => fun H : e |- U = V : T => consistent e)
+  (P0 := fun e T U s => fun H : e |- T >> U : s => consistent e) ;
+  simpl ; intros ; auto with coc.
+
+  apply consistent_cons with s ; auto with coc.
+  apply consistent_cons with s ; auto with coc.
+
+  apply consistent_cons with s' ; auto with coc.
+  apply consistent_cons with s ; auto with coc.
+Qed.
+
+Lemma typ_consistent : forall e t T, e |- t : T -> consistent e.
+Proof (proj1 consistency_ind).
+
+Lemma jeq_consistent : forall e U V T, e |- U = V : T -> consistent e.
+Proof (proj2 (proj2 consistency_ind)).
+
+Lemma coerce_consistent : forall e T U s, e |- T >> U : s -> consistent e.
+Proof (proj1 (proj2 consistency_ind)).
+
+
+
+Hint Resolve coerce_prop_prop coerce_set_set coerce_is_prop : coc.
+Hint Resolve lift_sort left_not_kind : coc.
