proof/JRussell/Freevars.v
@@ -1,0 +1,170 @@
+Require Import Lambda.Terms.
+Require Import Lambda.LiftSubst.
+Require Import Lambda.Reduction.
+Require Import Lambda.Conv.
+Require Import Lambda.Env.
+Require Import JRussell.Types.
+
+Set Implicit Arguments.
+
+Implicit Types i k m n p : nat.
+Implicit Type s : sort.
+Implicit Types A B M N T t u v : term.
+
+Lemma free_db_lift1_rec : forall n t, free_db n t -> forall k, free_db (S n) (lift_rec 1 t k).
+Proof.
+  simple induction 1 ; simpl ; intros ; auto with coc core arith datatypes.
+
+  elim (le_gt_dec k0 n0) ; simpl ; intros ;
+  constructor ; auto with arith.
+Qed.
+
+Lemma free_db_lift1 : forall n t, free_db n t -> free_db (S n) (lift 1 t).
+Proof.
+  unfold lift ; intros ; apply free_db_lift1_rec ; assumption.
+Qed.
+
+Hint Resolve free_db_lift1 : coc.
+
+Lemma free_db_lift_rec : forall n t, free_db n t -> forall n' k, free_db (n' + n) (lift_rec n' t k).
+Proof.
+  assert(forall n' k, S (n' + k) = n' + S k) ; try (intros ; omega). 
+  simple induction 1 ; simpl ; intros ; try constructor ; try rewrite H ; auto with coc core arith datatypes.
+
+  elim (le_gt_dec k0 n0) ; simpl ; intros ;
+  constructor ; auto with arith.
+  omega.
+Qed.
+
+Require Import Omega.
+Require Import Arith.
+
+Lemma term_free_db : forall e t T, e |- t : T -> free_db (length e) t.
+Proof.
+  simple induction 1 ; intros ; auto with coc core arith datatypes.
+
+  simpl.
+  constructor.
+  auto with arith.
+
+  simpl ; apply free_db_lift1.
+  assumption.
+Qed.
+
+Hint Resolve term_free_db : coc.
+
+  Lemma free_db_subst_rec : forall t n, free_db (S n) t -> 
+    forall m t', free_db m t' -> n >= m -> free_db n (subst_rec t' t (n - m)).
+Proof.
+
+  assert(Hsnk : forall n k, S (n + k) = n + S k) ; try (intros ; omega). 
+  induction t ; simpl ; intros ; try inversion H ; try constructor ; try rewrite Hsnk ; auto with coc core arith datatypes.
+  
+  elim (lt_eq_lt_dec (n0 - m) n) ; simpl ; intros ; 
+  auto with arith.
+  destruct a.
+  constructor ; auto with arith.
+  inversion H.
+  omega.
+  unfold lift.
+  pose (free_db_lift_rec).
+  rewrite e.
+   pose (f m t' H0 n).
+  assert(n0 = n + m) ; try omega.
+  rewrite H5.
+  apply f0.
+  
+  constructor.
+  omega.
+  
+  assert(S (n - m) = (S n) - m) ; try omega.
+  rewrite H7.
+  apply IHt2 ; auto.
+
+  assert(S (n - m) = (S n) - m) ; try omega.
+  rewrite H7.
+  apply IHt2 ; auto.
+
+  assert(S (n - m) = (S n) - m) ; try omega.
+  rewrite H7.
+  apply IHt2 ; auto.
+
+  assert(S (n - m) = (S n) - m) ; try omega.
+  rewrite H7.
+  apply IHt2 ; auto.
+Qed.
+
+
+Lemma free_db_subst : forall t n, free_db (S n) t -> 
+ forall t', free_db n t'-> free_db n (subst t' t).
+Proof.
+  unfold subst ; intros.
+  assert(n - n = 0) ; try omega.
+  rewrite <- H1.
+  apply free_db_subst_rec ; auto with arith.
+Qed.
+
+Lemma type_free_db : 
+  (forall e t T, e |- t : T -> free_db (length e) T) /\
+  (forall e U V s, e |- U >> V : s -> free_db (length e) U /\ free_db (length e) V) /\
+  (forall e U V T, e |- U = V : T -> free_db (length e) U /\ free_db (length e) V).
+Proof.
+  apply typ_coerce_jeq_ind with
+  (P:= fun e t T => fun H : e |- t : T => free_db (length e) T)
+  (P0:= fun e U V s => fun H : e |- U >> V : s => free_db (length e) U /\ free_db (length e) V)
+  (P1 := fun e U V T => fun H : e |- U = V : T => free_db (length e) U /\ free_db (length e) V) ;
+  simpl ; intros ; intuition ; try constructor ; try (apply (term_free_db t)) ; auto with coc core arith datatypes.
+
+  apply free_db_lift1 ;  apply term_free_db with (Srt s) ; auto.
+
+  inversion H0.
+  pose (term_free_db t).
+  apply free_db_subst ; auto.
+  
+  apply (term_free_db t1).
+
+  inversion H.
+  assumption.
+  
+  inversion H.
+  pose (term_free_db t0).
+  assert(free_db (length e) (Pi1 t)).
+  constructor ; auto.
+  apply free_db_subst ; auto.
+
+
+  apply (term_free_db t1).
+
+  apply (term_free_db t1).
+
+  constructor ; auto.
+  apply (term_free_db t1).
+  apply (term_free_db t2).
+  
+  apply free_db_subst ; auto.
+  apply (term_free_db t1).
+  apply (term_free_db t2).
+
+  constructor ; auto.
+  constructor ; auto.
+  apply (term_free_db t0).
+  apply (term_free_db t1).
+  apply (term_free_db t2).
+  apply (term_free_db t1).
+  
+  constructor ; auto.
+  constructor ; auto.
+  apply (term_free_db t0).
+  apply (term_free_db t1).
+  apply (term_free_db t2).
+  apply (term_free_db t2).
+Qed.
+
+Lemma typ_free_db : forall e t T, e |- t : T -> free_db (length e) T.
+Proof (proj1 (type_free_db)).
+
+Lemma coerce_free_db : forall e T U s, e |- T >> U : s -> free_db (length e) T /\ free_db (length e) U.
+Proof (proj1 (proj2 (type_free_db))).
+
+Lemma jeq_free_db : forall e U V T , e |- U = V : T -> free_db (length e) U /\ free_db (length e) V.
+Proof (proj2 (proj2 (type_free_db))).
