proof/JRussell/Thinning.v
@@ -1,0 +1,411 @@
+Require Import Lambda.Terms.
+Require Import Lambda.Reduction.
+Require Import Lambda.LiftSubst.
+Require Import Lambda.Env.
+Require Import Lambda.Conv.
+Require Import JRussell.Types.
+
+Set Implicit Arguments.
+
+Implicit Types i k m n p : nat.
+Implicit Type s : sort.
+Implicit Types A B M N T t u v : term.
+Implicit Types e f g : env.
+
+Lemma type_weak_lift_rec : forall e t T, e |- t : T -> forall A s, e |- A : Srt s ->
+  (A :: e) |- lift_rec 1 t 0 : lift_rec 1 T 0. 
+Proof.
+  intros.
+  pose (type_weak H H0).
+  unfold lift in t0.
+  apply t0.
+Qed.
+
+Lemma coerce_weak_lift_rec : forall e T U s, e |- T >> U : s -> forall A s', e |- A : Srt s' ->
+  (A :: e) |- lift_rec 1 T 0 >> lift_rec 1 U 0 : s. 
+Proof.
+  intros.
+  pose (coerce_weak H H0).
+  unfold lift in c.
+  apply c.
+Qed.
+
+Lemma jeq_weak_lift_rec : forall e t u T, e |- t = u : T -> forall A s, e |- A : Srt s ->
+  (A :: e) |- lift_rec 1 t 0 = lift_rec 1 u 0 : lift_rec 1 T 0. 
+Proof.
+  intros.
+  pose (jeq_weak H H0).
+  unfold lift in j.
+  apply j.
+Qed.
+
+Hint Resolve type_weak_lift_rec : coc.
+
+Lemma ind_weak_weak : forall g A s, g |- A : Srt s ->
+  (forall e t T, e |- t : T ->
+   forall n f, ins_in_env A n e f ->
+   trunc _ n e g ->
+   f |- (lift_rec 1 t n) : (lift_rec 1 T n)) /\
+ (forall e T U s, e |- T >> U : s ->
+  forall n f, ins_in_env A n e f ->
+  trunc _ n e g ->
+  f |- (lift_rec 1 T n) >> (lift_rec 1 U n) : s) /\
+ (forall e U V T, e |- U = V : T ->
+  forall n f, ins_in_env A n e f ->
+  trunc _ n e g ->
+  f |- (lift_rec 1 U n) = (lift_rec 1 V n) : (lift_rec 1 T n)).
+Proof.
+intros g A As HAs.
+apply typ_coerce_jeq_ind with 
+ (P := fun e t T => fun IH : typ e t T =>
+   forall n f, ins_in_env A n e f ->
+   trunc _ n e g -> 
+   f |- (lift_rec 1 t n) : (lift_rec 1 T n))
+ (P0 := fun e T U s => fun IH : coerce e T U s =>
+  forall n f, ins_in_env A n e f ->
+  trunc _ n e g ->
+  f |- (lift_rec 1 T n) >> (lift_rec 1 U n) : s)
+ (P1 := fun e U V T => fun IH : e |- U = V : T =>
+  forall n f, ins_in_env A n e f ->
+  trunc _ n e g -> 
+  f |- (lift_rec 1 U n) = (lift_rec 1 V n) : (lift_rec 1 T n)) ; 
+  intros ; try simpl in H ; try simpl in H0 ; try simpl in H1 ; try simpl in H2 ; try simpl in H3 ; 
+  try simpl in H4 ; 
+  auto with coc core arith datatypes.
+(* Prop *)
+inversion H.
+inversion H0.
+rewrite <- H6 in HAs.
+apply type_weak_lift_rec with As ; auto with coc.
+
+(* Set *)
+inversion H.
+inversion H0.
+rewrite <- H6 in HAs.
+apply type_weak_lift_rec with As ; auto with coc.
+
+(* Var *)
+inversion H0.
+rewrite <- H2 in H1.
+inversion H1.
+apply type_weak_lift_rec with As ; auto with coc.
+apply type_var with s ; auto with coc.
+rewrite H7 ; assumption.
+
+simpl.
+rewrite <- permute_lift.
+apply type_var with s ; auto with coc.
+simpl in H.
+rewrite <- H3 in H1.
+inversion H1.
+apply H ; auto with coc.
+
+(* Weak *)
+inversion H1.
+rewrite <- H3 in H2.
+inversion H2.
+apply type_weak_lift_rec with As ; auto with coc.
+apply type_weak with s ; auto with coc.
+rewrite H8 ; assumption.
+rewrite <- H4 in H2.
+inversion H2.
+rewrite <- permute_lift.
+rewrite <- permute_lift.
+apply type_weak with s ; auto with coc.
+
+(* Abs *)
+simpl.
+apply type_abs with s1 s2 ; auto with coc.
+
+(* App *)
+simpl.
+rewrite distr_lift_subst.
+apply type_app with (lift_rec 1 V n) ; auto with coc.
+
+(* Pair *)
+simpl.
+apply type_pair with s1 s2 s3 ; auto with coc.
+rewrite <- distr_lift_subst ; auto with coc.
+
+(* Prod *)
+simpl.
+apply type_prod with s1 ; auto with coc.
+
+(* Sum *)
+simpl.
+apply type_sum with s1 s2 ; auto with coc.
+
+(* Subset *)
+simpl.
+apply type_subset ; auto with coc.
+
+(* Pi1 *)
+simpl.
+apply type_pi1 with (lift_rec 1 V (S n)) ; auto with coc.
+
+(* Pi2 *)
+simpl.
+rewrite distr_lift_subst.
+simpl.
+apply type_pi2 with (lift_rec 1 U n) ; auto with coc.
+
+(* Conv *)
+apply type_conv with (lift_rec 1 U n) s ; auto with coc.
+
+(** coercion *)
+(* Conv done *)
+
+(* Weak *)
+inversion H1.
+rewrite <- H3 in H2.
+inversion H2.
+apply coerce_weak_lift_rec with As ; auto with coc.
+apply coerce_weak with s' ; auto with coc.
+rewrite H8 ; assumption.
+rewrite <- H4 in H2.
+inversion H2.
+rewrite <- permute_lift.
+rewrite <- permute_lift.
+apply coerce_weak with s' ; auto with coc.
+
+(* Prod *)
+simpl.
+apply coerce_prod with s ; auto with coc.
+
+(* Sum *)
+simpl.
+apply coerce_sum with s s' ; auto with coc.
+
+(* Subset left *)
+simpl.
+apply coerce_sub_l ; auto with coc.
+
+(* Subset right *)
+simpl.
+apply coerce_sub_r ; auto with coc.
+
+(* Sym done *)
+
+(* Trans *)
+apply coerce_trans with (lift_rec 1 B n) ; auto with coc.
+
+(** Judgemental equality *)
+(* Weak *)
+inversion H1.
+rewrite <- H3 in H2.
+inversion H2.
+apply jeq_weak_lift_rec with As ; auto with coc.
+apply jeq_weak with s ; auto with coc.
+rewrite H8 ; assumption.
+rewrite <- H4 in H2.
+inversion H2.
+do 3 rewrite <- permute_lift.
+apply jeq_weak with s ; auto with coc.
+
+(* Prod *)
+simpl ; apply jeq_prod with s1 ; auto with coc.
+
+(* Abs *)
+simpl ; apply jeq_abs with s1 s2 ; auto with coc.
+
+(* App *)
+rewrite distr_lift_subst.
+simpl ; apply jeq_app with (lift_rec 1 A0 n) ; auto with coc.
+
+(* Beta *)
+do 2 rewrite distr_lift_subst.
+simpl ; apply jeq_beta with s1 s2 ; auto with coc.
+
+(* Red *)
+apply jeq_red with (lift_rec 1 A0 n) s ; auto with coc.
+
+(* Exp *)
+apply jeq_exp with (lift_rec 1 B n) s ; auto with coc.
+
+(* Sum *)
+simpl ; apply jeq_sum with s1 s2 ; auto with coc.
+
+(* Pair *)
+simpl ; apply jeq_pair with s1 s2 s3 ; auto with coc.
+simpl.
+rewrite <- distr_lift_subst.
+apply H2 ; auto with coc.
+
+(* Pi1 *)
+simpl ; apply jeq_pi1 with (lift_rec 1 B (S n)) ; auto with coc.
+
+(* Pi1 red *)
+simpl ; apply jeq_pi1_red with s1 s2 s3 ; auto with coc.
+rewrite <- distr_lift_subst.
+apply H2 ; auto with coc.
+
+(* Pi2 *)
+rewrite distr_lift_subst.
+simpl ; apply jeq_pi2 with (lift_rec 1 A0 n) ; auto with coc.
+
+(* Pi2 red *)
+rewrite distr_lift_subst.
+simpl ; apply jeq_pi2_red with s1 s2 s3; auto with coc.
+rewrite <- distr_lift_subst.
+apply H2 ; auto with coc.
+
+(* Subset *)
+simpl ; apply jeq_subset ; auto with coc.
+
+(* Trans *)
+simpl; apply jeq_trans with (lift_rec 1 N n) ; auto with coc.
+
+(* Conv *)
+simpl ; apply jeq_conv with (lift_rec 1 A0 n) s ; auto with coc.
+Qed.
+
+Lemma type_weak_weak : forall g A s, g |- A : Srt s ->
+  forall e t T, e |- t : T ->
+   forall n f, ins_in_env A n e f ->
+   trunc _ n e g ->
+   f |- (lift_rec 1 t n) : (lift_rec 1 T n).
+Proof.
+  intros g A s H.
+  exact (proj1 (ind_weak_weak H)).
+Qed.
+
+Lemma coerce_weak_weak : forall g A s, g |- A : Srt s ->
+  forall e T U s, e |- T >> U : s ->
+  forall n f, ins_in_env A n e f ->
+  trunc _ n e g ->
+  f |- (lift_rec 1 T n) >> (lift_rec 1 U n) : s.
+Proof.
+  intros g A s H.
+  exact (proj1 (proj2 (ind_weak_weak H))).
+Qed.
+
+Lemma jeq_weak_weak : forall g A s, g |- A : Srt s ->
+  forall e U V T, e |- U = V : T ->
+  forall n f, ins_in_env A n e f ->
+  trunc _ n e g ->
+  f |- (lift_rec 1 U n) = (lift_rec 1 V n) : (lift_rec 1 T n).
+Proof.
+  intros g A s H.
+  exact (proj2 (proj2 (ind_weak_weak H))).
+Qed.
+
+Lemma thinning_n :
+   forall n e f,
+   trunc _ n e f ->
+   consistent e ->
+   forall t T, typ f t T -> typ e (lift n t) (lift n T).
+Proof.
+simple induction n.
+intros.
+rewrite lift0.
+rewrite lift0.
+replace e with f; auto with coc core arith datatypes.
+inversion_clear H; auto with coc core arith datatypes.
+
+do 8 intro.
+inversion H0.
+intro.
+rewrite simpl_lift; auto with coc core arith datatypes.
+pattern (lift (S n0) T) in |- *.
+rewrite simpl_lift; auto with coc core arith datatypes.
+rewrite <- H4 in H1.
+inversion H1.
+apply type_weak with s ; auto with coc.
+apply H with f ; auto.
+Qed.
+
+Lemma thinning_n_coerce : forall n e f, trunc _ n e f -> 
+  forall T U s, f |- T >> U : s -> consistent e -> e |- (lift n T) >> (lift n U) : s.
+Proof.
+simple induction n.
+intros.
+rewrite lift0.
+rewrite lift0.
+replace e with f; auto with coc core arith datatypes.
+inversion_clear H; auto with coc core arith datatypes.
+
+do 9 intro.
+inversion_clear H0.
+intro.
+rewrite simpl_lift; auto with coc core arith datatypes.
+pattern (lift (S n0) T) in |- *.
+rewrite simpl_lift; auto with coc core arith datatypes.
+inversion_clear H0.
+replace (lift (S n0) U) with (lift 1 (lift n0 U)).
+apply coerce_weak with s0 ; auto with coc.
+eapply H with f ; auto with coc core arith datatypes.
+rewrite <- simpl_lift.
+auto.
+Qed.
+
+Hint Resolve thinning_n thinning_n_coerce : coc.
+
+Lemma item_ref_lift :
+ forall n e t, item _ t e n -> consistent e -> e |- Ref n : lift (S n) t.
+simple induction n ; intros.
+inversion H.
+rewrite <- H1 in H0.
+inversion H0.
+apply type_var with s ; auto.
+
+inversion H0.
+change (Ref (S n0)) with (lift 1 (Ref n0)).
+replace (lift (S (S n0)) (t)) with (lift 1 (lift (S n0) t)).
+apply thinning_n with l ; try constructor ; auto with coc.
+rewrite H3 ; auto.
+apply H ; auto.
+rewrite <- H3 in H1.
+inversion H1.
+auto.
+rewrite <- simpl_lift.
+reflexivity.
+Qed.
+
+(*Lemma item_sorted_lift :
+ forall e n t, item _ t e n -> 
+ forall f, trunc _ n e f -> exists s : sort, f |- t : (Srt s).
+intros e u V H.
+simple induction n ; intros.
+
+inversion H0.
+rewrite <- H2 in H1.
+inversion H1.
+rewrite <- H2 in H.
+inversion H.
+exists 
+
+simple destruct e; intros.
+elim H0; intros.
+inversion_clear H2.
+
+elim H0; intros.
+rewrite H1.
+inversion_clear H2.
+inversion_clear H.
+exists s.
+replace (Srt s) with (lift 1 (Srt s)); auto with coc core arith datatypes.
+apply thinning; auto with coc core arith datatypes.
+apply wf_var with s; auto with coc core arith datatypes.
+
+intros.
+elim H1; intros.
+rewrite H2.
+generalize H0.
+inversion_clear H3; intros.
+rewrite simpl_lift; auto with coc core arith datatypes.
+cut (wf l); intros.
+elim H with l (lift (S n0) x); intros; auto with coc core arith datatypes.
+inversion_clear H3.
+exists x0.
+change (typ (y :: l) (lift 1 (lift (S n0) x)) (lift 1 (Srt x0))) in |- *.
+apply thinning; auto with coc core arith datatypes.
+apply wf_var with s; auto with coc core arith datatypes.
+
+exists x; auto with coc core arith datatypes.
+
+inversion_clear H3.
+apply typ_wf with y (Srt s); auto with coc core arith datatypes.
+Qed.
+
+
+*)
