proof/JRussell/Validity.v
@@ -1,0 +1,561 @@
+Require Import Lambda.Terms.
+Require Import Lambda.Reduction.
+Require Import Lambda.Conv.
+Require Import Lambda.Conv_Dec.
+Require Import Lambda.LiftSubst.
+Require Import Lambda.Env.
+Require Import JRussell.Types.
+Require Import JRussell.Basic.
+Require Import JRussell.Conversion.
+Require Import JRussell.Coercion.
+Require Import JRussell.Thinning.
+Require Import JRussell.Substitution.
+Require Import JRussell.PreFunctionality.
+Require Import JRussell.Generation.
+
+Implicit Types i k m n p : nat.
+Implicit Type s : sort.
+Implicit Types A B M N T t u v : term.
+Implicit Types e f g : env.
+
+Set Implicit Arguments.
+
+Lemma app_cons_app_app : forall e' a e, e' ++ a :: e = (e' ++ a :: nil) ++ e.
+Proof.
+  induction e' ; simpl ; intros ; auto.
+  rewrite IHe'.
+  reflexivity.
+Qed.
+
+Lemma strength_sort_judgement : forall e s s', e |- Srt s : Srt s' -> nil |- Srt s : Srt s'.
+Proof.
+  intros.
+  destruct s.
+  elim left_not_kind with e (Srt kind) (Srt s') ; auto.
+
+  pose (generation_sort H).
+  pose (equiv_kind e0).
+  rewrite e1.
+  auto with coc.
+
+  pose (generation_sort H).
+  pose (equiv_kind e0).
+  rewrite e1.
+  auto with coc.
+Qed.
+
+Lemma trunc_list : forall e, trunc _ (length e) e nil.
+Proof.
+  induction e ; simpl ;
+  constructor ; auto.
+Qed.
+
+Lemma sort_judgement_empty_env : forall s s', nil |- Srt s : Srt s' ->
+  forall e, consistent e -> e |- Srt s : Srt s'.
+Proof.
+  intros.
+  pose (thinning_n (trunc_list e) H0 H). 
+  unfold lift in t ; simpl in t.
+  assumption.
+Qed.
+
+Lemma weak_one_sort_judgement : forall T e s s', T :: e |- Srt s : Srt s' -> 
+  e |- Srt s : Srt s'.
+Proof.
+  intros.
+  pose (typ_consistent H).
+  pose (strength_sort_judgement H).
+  inversion c.
+  apply (sort_judgement_empty_env t H2).
+Qed.
+
+Hint Resolve weak_one_sort_judgement : coc.
+
+Lemma validity_ind : 
+  (forall e t T, e |- t : T ->
+  T = Srt kind \/ exists s, e |- T : Srt s) /\
+  (forall e T U s, e |- T >> U : s ->
+  e |- T : Srt s /\ e |- U : Srt s) /\
+  (forall e t u T, e |- t = u : T ->
+  (e |- t : T /\ e |- u : T) /\
+  (T = Srt kind \/ exists s, e |- T : Srt s)).
+Proof.
+  apply typ_coerce_jeq_ind with 
+  (P := fun e t T => fun H : e |- t : T =>
+  T = Srt kind \/ exists s, e |- T : Srt s)
+  (P0 := fun e T U s => fun H : e |- T >> U : s =>
+  e |- T : Srt s /\ e |- U : Srt s)
+  (P1 := fun e t u T => fun H : e |- t = u : T =>
+  (e |- t : T /\ e |- u : T) /\
+  (T = Srt kind \/ exists s, e |- T : Srt s)) ;
+  simpl ; intros ; auto with coc ; try discriminate ; 
+  try (destruct H ; discriminate) ;  try (destruct H1 ; discriminate).
+
+  destruct H.
+  right.
+  inversion H.
+  rewrite H1 in t.
+  exists kind.
+  change (Srt kind) with (lift 1 (Srt kind)).
+  apply type_weak with kind ; auto with coc.
+  
+  destruct H.
+  pose (generation_sort H).
+  right.
+  exists s.
+  change (Srt s) with (lift 1 (Srt s)).
+  apply type_weak with s ; auto with coc.
+
+  destruct H.
+  left ; rewrite H ; auto with coc.
+
+  destruct H.
+  right.
+  exists x.
+  change (Srt x) with (lift 1 (Srt x)).
+  apply type_weak with s ; auto with coc.
+
+  right.
+  exists s2 ; apply type_prod with s1 ; auto with coc.
+
+  destruct H0 ; try discriminate.
+  destruct H0.
+  right.
+  pose (generation_prod H0).
+  destruct e0.
+  destruct H1.
+  destruct H1.
+  destruct H2.
+
+  exists x1.
+  change (Srt x1) with (subst v (Srt x1)).
+  apply substitution with V ; auto with coc.
+
+  right.
+  exists s3 ; apply type_sum with s1 s2 ; auto with coc.
+
+  destruct H0.
+  left ; auto.
+  destruct H0.
+  right.
+  exists x.
+  inversion H0.
+  rewrite H3 ; rewrite H4.
+  apply weak_one_sort_judgement with T ; assumption.
+  apply weak_one_sort_judgement with T; assumption.
+  
+  right.
+  pose (typ_consistent t).
+  exists kind.
+  apply sort_judgement_empty_env ; auto.
+  destruct s;
+  destruct H1 ; destruct H2 ; rewrite H3 ; auto with coc.
+
+  destruct H ; try discriminate.
+  destruct H.
+  pose (generation_sum H).
+  destruct e0.
+  do 2 destruct H0.
+  intuition.
+  right ; exists x0 ; assumption.
+
+  destruct H ; try discriminate.
+  destruct H.
+  pose (generation_sum H).
+  destruct e0.
+  do 2 destruct H0.
+  intuition.
+  right ; exists x1 ; auto with coc.
+  change (Srt x1) with (subst (Pi1 t) (Srt x1)).
+  apply substitution with U ; auto with coc.
+  apply type_pi1 with V ; auto with coc.
+
+  destruct H.
+  destruct H0 ; try contradiction.
+  destruct H.
+  right ; exists s ; auto.
+
+  right ; intuition.
+
+  exists s ; intuition.
+
+  destruct H ; intuition.
+
+  destruct H.
+  change (Srt s) with (lift 1 (Srt s)).
+  split ; apply type_weak with s' ; auto.
+
+  split ; apply type_prod with s ; auto with coc.
+
+  split ; apply type_sum with s s' ; auto with coc.
+
+  split ; auto with coc ; apply type_subset ; auto with coc.
+
+  split ; auto with coc ; apply type_subset ; auto with coc.
+
+  intuition.
+
+  intuition.
+
+  (* Judgemental equality *)
+  destruct H.
+  destruct H.
+  split.
+  split ; apply type_weak with s ; auto with coc.
+
+  destruct H1.
+  rewrite H1 ; left ; auto.
+  destruct H1.
+  right ; exists x ; change (Srt x) with (lift 1 (Srt x)) ; 
+  apply type_weak with s ; auto with coc.
+
+  (* Prod *)
+  do 2 destruct H.
+  do 2 destruct H0.
+  split.
+  split ; apply type_prod with s1 ; auto with coc.
+  apply (type_conv_env H4).
+  apply conv_env_hd with s1 ; auto with coc.
+
+  destruct H3.
+  left ; auto.
+  right.
+  destruct H3.
+  exists x.
+  apply weak_one_sort_judgement with U ; auto.
+
+  (* Abs *)  
+  do 2 destruct H.
+  do 2 destruct H1.
+  split.
+  split ; try apply type_abs with s1 s2 ; auto with coc.
+  assert(conv_in_env (A :: e) (A' :: e)).
+  apply conv_env_hd with s1 ; auto with coc.
+  pose (type_conv_env H5 H6).
+  apply type_conv with (Prod A' B) s2 ; auto with coc.
+  apply type_abs with s1 s2 ; auto with coc.
+  apply (type_conv_env t H6).
+  apply coerce_prod with s1 ; auto with coc.
+  apply (type_conv_env t H6).
+  
+  right.
+  exists s2 ; apply type_prod with s1 ; auto with coc.
+  
+  (* App *)
+  do 2 destruct H.
+  do 2 destruct H0.
+  destruct H1 ; try discriminate.
+  destruct H1.
+  pose (generation_prod H1).
+  destruct e0.
+  do 2 destruct H5.
+  destruct H6.
+  split.
+  split ; try apply type_app with A ; auto with coc.
+  apply type_conv with (subst N' B) x1 ; auto with coc.
+  apply type_app with A ; auto with coc.
+  apply coerce_conv ; auto with coc.
+  change (Srt x1) with (subst N (Srt x1)).
+  apply jeq_sym.
+  apply pre_functionality with A ; auto with coc.
+
+  right ; exists x1.
+  change (Srt x1) with (subst N (Srt x1)).
+  apply substitution with A ; auto with coc.
+
+  (* Beta *)
+  split.
+  split ; try apply type_app with A ; auto with coc.
+  apply type_abs with s1 s2 ; auto with coc.
+  apply substitution with A ; auto.
+
+  right.
+  exists s2.
+  change (Srt s2) with (subst N (Srt s2)).
+  apply substitution with A ; auto with coc.
+
+  (* Red *)
+  do 2 destruct H0.
+  do 2 destruct H.
+  split.
+  split ; apply type_conv with A s ; auto with coc.
+
+  right.
+  exists s ; auto.
+
+  (* Exp *)
+  do 2 destruct H0.
+  do 2 destruct H.
+  split.
+  split ; apply type_conv with B s ; auto with coc.
+
+  right.
+  exists s ; auto.
+
+  (* Sum *)
+  do 2 destruct H.
+  do 2 destruct H0.
+  split.
+  split ; apply type_sum with s1 s2 ; auto with coc.
+  apply (type_conv_env H4).
+  apply conv_env_hd with s1 ; auto with coc.
+
+  right ; exists kind.
+  pose (typ_consistent H).
+  apply sort_judgement_empty_env ; auto with coc.
+  
+  inversion s ;
+  destruct H5 ;
+  destruct H6 ;
+  try rewrite H7 ; auto with coc.
+
+  (* Pair *)  
+  do 2 destruct H.
+  do 2 destruct H0.
+  do 2 destruct H1.
+  do 2 destruct H2.
+  split.
+  split ; try apply type_pair with s1 s2 s3 ; auto with coc.
+  apply type_conv with (Sum A' B') s3; auto with coc.
+  apply type_pair with s1 s2 s3 ; auto with coc.
+  apply type_conv with A s1 ; auto with coc.
+  assert(conv_in_env (A :: e) (A' :: e)).
+  apply conv_env_hd with s1 ; auto with coc.
+  apply (type_conv_env H6 H11).
+  
+  apply type_conv with (subst u B) s2 ; auto with coc.
+  apply coerce_conv ; auto with coc.
+  apply jeq_trans with (subst u' B) ; auto with coc.
+  change (Srt s2) with (subst u (Srt s2)).
+  apply pre_functionality with A ; auto with coc.
+  change (Srt s2) with (subst u' (Srt s2)).
+  apply substitution_jeq with A ; auto with coc.
+
+  apply coerce_conv ; auto with coc.
+  apply jeq_sum with s1 s2 ; auto with coc.
+  apply jeq_sym.
+  apply jeq_conv_env with (A :: e) ; auto with coc.
+  apply conv_env_hd with s1 ; auto with coc.
+
+  right.
+  exists s3 ; apply type_sum with s1 s2 ; auto with coc.
+
+  (* Pi1 *)
+  do 2 destruct H.
+  split ; try (split ; apply type_pi1 with B ; auto with coc).
+  right.
+  destruct H0 ; try discriminate.
+  destruct H0.
+  pose (generation_sum H0).
+  destruct e0.
+  do 3 destruct H2.
+  exists x0 ; auto.
+
+  (* Pi1 red *)
+  split.
+  split ; auto.
+  apply type_pi1 with B ; auto with coc.
+  apply type_pair with s1 s2 s3 ; auto with coc.
+  right ; exists s1 ; assumption.
+
+  (* Pi2 *)
+  do 2 destruct H.
+  destruct H0 ; try discriminate.
+  destruct H0.
+  pose (generation_sum H0).
+  destruct e0.
+  do 3 destruct H2.
+  split.
+  split. 
+  apply type_pi2 with A ; auto with coc.
+  apply type_conv with (subst (Pi1 t') B) x1.
+  apply type_pi2 with A ; auto with coc.
+  intuition.
+  apply coerce_conv ; auto.
+  change (Srt x1) with (subst (Pi1 t) (Srt x1)).
+  apply jeq_sym.
+  apply pre_functionality with A ; auto with coc.
+  apply type_pi1 with B ; auto with coc.
+  apply jeq_pi1 with B ; auto with coc.
+
+  right.
+  exists x1 ; intuition ; auto.
+  change (Srt x1) with (subst (Pi1 t) (Srt x1)).
+  apply substitution with A ; auto with coc.
+  apply type_pi1 with B ; auto with coc.
+
+  (* Pi2 red *)
+  split.
+  split ; auto.
+  apply type_conv with (subst (Pi1 (Pair (Sum A B) u v)) B) s2 ; auto with coc.
+  apply type_pi2 with A ; auto with coc.
+  apply type_pair with s1 s2 s3 ; auto with coc.
+  apply coerce_conv ; auto.
+  change (Srt s2) with (subst (Pi1 (Pair (Sum A B) u v)) (Srt s2)).
+  apply pre_functionality with A ; auto with coc.
+  apply type_pi1 with B ; auto with coc.
+  apply type_pair with s1 s2 s3 ; auto with coc.
+  
+  apply jeq_pi1_red with s1 s2 s3 ; auto with coc.
+
+  right.
+  exists s2.
+  change (Srt s2) with (subst u (Srt s2)).
+  apply substitution with A ; auto with coc.
+
+  (* Subset *)
+  do 2 destruct H.
+  do 2 destruct H0.
+  split.
+  split ; try apply type_subset ; auto with coc.
+  
+  apply type_conv_env with (A :: e) ; auto with coc.
+  apply conv_env_hd with set ; auto.
+  right.
+  exists kind.
+  apply sort_judgement_empty_env ; auto with coc.
+  apply (typ_consistent H).
+
+  (* Sym *)
+  do 2 destruct H.
+  split ; try (split ; auto) ; auto.
+
+  (* Trans *)
+  do 2 destruct H.
+  do 2 destruct H0.
+  split ; auto.
+
+  (* Coerce *)
+  do 2 destruct H.
+  destruct H0.
+  split ; auto.
+  split ; apply type_conv with A s ; auto.
+  right.
+  exists s ; assumption.
+Qed.
+
+Lemma validity_typ :
+  forall e t T, e |- t : T ->
+  T = Srt kind \/ exists s, e |- T : Srt s.
+Proof (proj1 validity_ind).
+
+Lemma validity_coerce :
+  forall e T U s, e |- T >> U : s ->
+  e |- T : Srt s /\ e |- U : Srt s.
+Proof (proj1 (proj2 validity_ind)).
+
+Lemma validity_jeq :
+ forall e t u T, e |- t = u : T ->
+ (e |- t : T /\ e |- u : T) /\
+ (T = Srt kind \/ exists s, e |- T : Srt s).
+Proof (proj2 (proj2 validity_ind)).
+
+Inductive conv_env : env -> env -> Prop :=
+  | conv_env_hd : forall e t u s, e |- t = u : Srt s -> conv_env (t :: e) (u :: e)
+  | conv_env_tl :
+      forall e f t, conv_in_env e f -> conv_env (t :: e) (t :: f).
+
+Lemma conv_env_conv_in_env : forall e e', conv_env e e' -> conv_in_env e e'.
+Proof.
+  induction 1.
+  pose (validity_jeq H).
+  destruct a.
+  destruct H0.
+  apply (Conversion.conv_env_hd) with s ; auto.
+  constructor ; auto.
+Qed.
+
+Lemma type_conv_env : forall e t T, e |- t : T -> 
+  forall f, conv_env e f -> f |- t : T.
+Proof.
+  intros.
+  apply Conversion.type_conv_env with e ; auto.
+  apply conv_env_conv_in_env ; auto.
+Qed.
+
+Lemma coerce_conv_env : forall e T U s, e |- T >> U : s -> 
+  forall f, conv_env e f -> f |- T >> U : s.
+Proof.
+  intros.
+  apply Conversion.coerce_conv_env with e ; auto.
+  apply conv_env_conv_in_env ; auto.
+Qed.
+
+Lemma jeq_conv_env : forall e U V T, e |- U = V : T ->
+  forall f, conv_env e f -> f |- U = V : T.
+Proof.
+  intros.
+  apply Conversion.jeq_conv_env with e ; auto.
+  apply conv_env_conv_in_env ; auto.
+Qed.
+
+Lemma functionality_rec : forall g (d : term) t, 
+  forall d', g |- d = d' : t ->
+  forall e U T, e |- U : T ->
+  forall f n, sub_in_env d t n e f -> trunc _ n f g -> 
+  f |- (subst_rec d U n) = (subst_rec d' U n) : (subst_rec d T n).
+Proof.
+  intros.
+  apply pre_functionality_rec with g t e; auto.
+  pose (validity_jeq H).
+  destruct a.
+  destruct H3.
+  assumption.
+Qed.
+
+Lemma functionality :forall e (d : term) t, e |- d : t -> 
+  forall d', e |- d = d' : t ->
+  forall U T, t :: e |- U : T ->
+  e |- (subst d U) = (subst d' U) : (subst d T).
+Proof.
+  intros.
+  unfold subst ; pose functionality_rec.
+  apply (@pre_functionality_rec e d t H d' H0 (t :: e) U T H1).
+  constructor.
+  constructor.
+Qed.
+
+Lemma jeq_type_l : forall e u v T, e |- u = v : T -> e |- u : T.
+Proof.
+  intros.
+  pose (validity_jeq H).
+  intuition.
+Qed.
+
+Lemma jeq_type_r : forall e u v T, e |- u = v : T -> e |- v : T.
+Proof.
+  intros.
+  pose (validity_jeq H).
+  intuition.
+Qed.
+
+Lemma coerce_sort_l : forall e U V s, e |- U >> V : s -> e |- U : Srt s.
+Proof.
+  intros.
+  pose (validity_coerce H).
+  intuition.
+Qed.
+
+Lemma coerce_sort_r : forall e U V s, e |- U >> V : s -> e |- V : Srt s.
+Proof.
+  intros.
+  pose (validity_coerce H).
+  intuition.
+Qed.
+
+Hint Resolve jeq_type_l jeq_type_r coerce_sort_l coerce_sort_r : coc.
+
+Lemma jeq_subst_par : forall e u u' v v' A B, e |- u = u' : A -> A :: e |- v = v' : B ->
+  e |- subst u v = subst u' v' : subst u B.
+Proof.
+  intros.
+  pose (jeq_type_l H).
+  pose (jeq_type_l H0).
+
+  apply jeq_trans with (subst u v') ; auto with coc.
+  apply substitution_jeq with A ; auto with coc.
+  apply functionality with A ; auto with coc.
+  apply (jeq_type_r H0).
+Qed.
+
+
