proof/TPOSR/TPOSR_Jeq.v
@@ -1,0 +1,170 @@
+Require Import Lambda.Terms.
+Require Import Lambda.Reduction.
+Require Import Lambda.Conv.
+Require Import Lambda.LiftSubst.
+Require Import Lambda.Env.
+
+Require Import JRussell.Types.
+Require Import JRussell.Basic.
+Require Import JRussell.Generation.
+Require Import JRussell.Thinning.
+Require Import JRussell.Validity.
+
+Require Import TPOSR.Terms.
+Require Import TPOSR.Reduction.
+Require Import TPOSR.Conv.
+Require Import TPOSR.LiftSubst.
+Require Import TPOSR.Env.
+Require Import TPOSR.Types.
+Require Import TPOSR.Unlab.
+
+Implicit Types i k m n p : nat.
+Implicit Type s : sort.
+Implicit Types A B M N T t u v : lterm.
+Implicit Types e f g : lenv.
+
+Set Implicit Arguments.
+
+Lemma item_unlab : forall n t e, item lterm t e n -> item term (|t|) (unlab_ctx e) n.
+Proof.
+  induction n ; simpl ; intros ; auto.
+  inversion H.
+  simpl.
+  constructor.
+  
+  inversion H.
+  simpl.
+  constructor.
+  apply IHn ; auto.
+Qed.
+
+Theorem unlab_sound  : 
+  (forall e u v T, e |- u -> v : T -> 
+  (unlab_ctx e) |- (|u|) = (|v|) : (|T|)) /\
+  (forall e, tposr_wf e -> 
+  (unlab_ctx e) |- Srt prop : Srt kind /\
+  (unlab_ctx e) |- Srt set : Srt kind /\
+  (forall A n, item_llift A e n -> 
+  (unlab_ctx e) |- Ref n : (|A|))).
+Proof.
+  apply ind_tposr_wf with 
+  (P := fun e u v T=>  fun H : e |- u -> v : T =>
+  (unlab_ctx e) |- (|u|) = (|v|) : (|T|))
+  (P0 := fun e => fun H : tposr_wf e =>
+  (unlab_ctx e) |- Srt prop : Srt kind /\
+  (unlab_ctx e) |- Srt set : Srt kind /\
+  (forall A n, item_llift A e n -> 
+  (unlab_ctx e) |- Ref n : (|A|))) ; simpl ; intros ; auto with coc.
+
+  intuition.
+
+  intuition.
+
+  intuition.
+
+  apply jeq_prod with s1 ; auto with coc.
+
+  apply jeq_abs with s1 s2 ; auto with coc.
+  apply (jeq_type_l H0).
+
+  rewrite lab_subst.
+  apply jeq_app with (|A|) ; auto.
+
+  do 2 rewrite lab_subst.
+  pose (jeq_type_l H).
+  pose (jeq_type_l H0).
+  pose (jeq_type_l H1).
+  pose (jeq_type_l H2).
+  
+  apply jeq_trans with (subst (|N |) (|M |)) ; auto with coc.
+  apply jeq_beta with s1 s2 ; auto with coc.
+  
+  apply jeq_subst_par with (|A|); auto with coc.
+
+  apply jeq_red with (|A|) s ; auto with coc.
+
+  apply jeq_exp with (|B|) s ; auto with coc.
+
+  apply jeq_subset ; auto with coc.
+
+  apply jeq_sum  with s1 s2 ; auto with coc.
+
+  apply jeq_pi1 with (|B|) ; auto with coc.
+
+  pose (jeq_type_l H).
+  pose (jeq_type_l H0).
+  pose (jeq_type_l H1).
+  pose (generation_pair t4).
+  destruct e0.
+  do 4 destruct H2.
+  intuition.
+  inversion H3.
+  apply jeq_pi1_red with s1 s2 s3 ; auto with coc.
+  rewrite H10 ; assumption.
+  rewrite H11 ; assumption.
+
+  rewrite lab_subst.
+  simpl.
+  apply jeq_pi2 with (|A|) ; auto with coc.
+
+  pose (jeq_type_l H).
+  pose (jeq_type_l H0).
+  pose (jeq_type_l H1).
+  pose (generation_pair t4).
+  destruct e0.
+  do 4 destruct H2.
+  intuition.
+  inversion H3.
+  rewrite lab_subst.
+  apply jeq_pi2_red with s1 s2 s3 ; auto with coc.
+  rewrite H10 ; assumption.
+  rewrite H11 ; assumption.
+
+  split ; auto with coc.
+  split ; auto with coc.
+  intros.
+  inversion H.
+  inversion H1.
+
+  split ; auto with coc.
+  apply sort_judgement_empty_env ; auto with coc.
+  apply consistent_cons with s ; auto with coc.
+  apply (jeq_consistent H).
+  apply (jeq_type_l H).
+
+  split.
+  apply sort_judgement_empty_env ; auto with coc.
+  apply consistent_cons with s ; auto with coc.
+  apply (jeq_consistent H).
+  apply (jeq_type_l H).
+
+  intros.
+  inversion H0.
+  rewrite H1.
+  rewrite lab_lift.
+  apply (item_ref_lift).
+  induction n.
+  inversion H2.
+  constructor.
+  constructor.
+  inversion H2.
+  apply (item_unlab H4).
+  
+  apply consistent_cons with s.
+  apply (jeq_consistent H).
+  apply (jeq_type_l H).
+Qed.
+
+Corollary unlab_sound_type : forall e u v T, e |- u -> v : T -> 
+  (unlab_ctx e) |- (|u|) = (|v|) : (|T|).
+Proof (proj1 (unlab_sound)).
+
+Corollary unlab_sound_wf :
+  (forall e, tposr_wf e -> 
+  (unlab_ctx e) |- Srt prop : Srt kind /\
+  (unlab_ctx e) |- Srt set : Srt kind /\
+  (forall A n, item_llift A e n -> 
+  (unlab_ctx e) |- Ref n : (|A|))).
+Proof (proj2 (unlab_sound)).
+
+
