proof/TPOSR/Types.v
@@ -93,6 +93,137 @@ with tposr : lenv -> lterm -> lterm -> lterm -> Prop :=
 
 where "G |- T -> U : s" := (tposr G T U s).
 
+Scheme tposr_wf_mutind := Induction for tposr Sort Prop
+with wf_tposr_mutind :=  Induction for tposr_wf Sort Prop.
+
+Check tposr_wf_mutind.
+
+Lemma ind_tposr_wf :
+forall
+         (P : forall (l : lenv) (l0 l1 l2 : lterm),
+              l |- l0 -> l1 : l2 -> Prop)
+         (P0 : forall l : lenv, tposr_wf l -> Prop),
+       (forall (e : lenv) (t : tposr_wf e),
+        P0 e t ->
+        forall (n : nat) (T : lterm) (i : item_llift T e n),
+        P e (Ref_l n) (Ref_l n) T (tposr_var t i)) ->
+       (forall (e : lenv) (t : tposr_wf e),
+        P0 e t -> P e (Srt_l set) (Srt_l set) (Srt_l kind) (tposr_set t)) ->
+       (forall (e : lenv) (t : tposr_wf e),
+        P0 e t -> P e (Srt_l prop) (Srt_l prop) (Srt_l kind) (tposr_prop t)) ->
+       (forall (e : lenv) (A A' : lterm) (s1 : sort)
+          (t : e |- A -> A' : Srt_l s1),
+        P e A A' (Srt_l s1) t ->
+        forall (B B' : lterm) (s2 : sort) (t0 : A :: e |- B -> B' : Srt_l s2),
+        P (A :: e) B B' (Srt_l s2) t0 ->
+        P e (Prod_l A B) (Prod_l A' B') (Srt_l s2) (tposr_prod t t0)) ->
+       (forall (e : lenv) (A A' : lterm) (s1 : sort)
+          (t : e |- A -> A' : Srt_l s1),
+        P e A A' (Srt_l s1) t ->
+        forall (B B' : lterm) (s2 : sort) (t0 : A :: e |- B -> B' : Srt_l s2),
+        P (A :: e) B B' (Srt_l s2) t0 ->
+        forall (M M' : lterm) (t1 : A :: e |- M -> M' : B),
+        P (A :: e) M M' B t1 ->
+        P e (Abs_l A M) (Abs_l A' M') (Prod_l A B) (tposr_abs t t0 t1)) ->
+       (forall (e : lenv) (A A' : lterm) (s1 : sort)
+          (t : e |- A -> A' : Srt_l s1),
+        P e A A' (Srt_l s1) t ->
+        forall (B B' : lterm) (s2 : sort) (t0 : A :: e |- B -> B' : Srt_l s2),
+        P (A :: e) B B' (Srt_l s2) t0 ->
+        forall (M M' : lterm) (t1 : e |- M -> M' : Prod_l A B),
+        P e M M' (Prod_l A B) t1 ->
+        forall (N N' : lterm) (t2 : e |- N -> N' : A),
+        P e N N' A t2 ->
+        P e (App_l B M N) (App_l B' M' N') (lsubst N B)
+          (tposr_app t t0 t1 t2)) ->
+       (forall (e : lenv) (A A' : lterm) (s1 : sort)
+          (t : e |- A -> A' : Srt_l s1),
+        P e A A' (Srt_l s1) t ->
+        forall (B B' : lterm) (s2 : sort) (t0 : A :: e |- B -> B' : Srt_l s2),
+        P (A :: e) B B' (Srt_l s2) t0 ->
+        forall (M M' : lterm) (t1 : A :: e |- M -> M' : B),
+        P (A :: e) M M' B t1 ->
+        forall (N N' : lterm) (t2 : e |- N -> N' : A),
+        P e N N' A t2 ->
+        P e (App_l B (Abs_l A M) N) (lsubst N' M') (lsubst N B)
+          (tposr_beta t t0 t1 t2)) ->
+       (forall (e : lenv) (M N A : lterm) (t : e |- M -> N : A),
+        P e M N A t ->
+        forall (B : lterm) (s : sort) (t0 : e |- A -> B : Srt_l s),
+        P e A B (Srt_l s) t0 -> P e M N B (tposr_red t t0)) ->
+       (forall (e : lenv) (M N B : lterm) (t : e |- M -> N : B),
+        P e M N B t ->
+        forall (A : lterm) (s : sort) (t0 : e |- A -> B : Srt_l s),
+        P e A B (Srt_l s) t0 -> P e M N A (tposr_exp t t0)) ->
+       (forall (e : lenv) (A A' : lterm) (t : e |- A -> A' : Srt_l set),
+        P e A A' (Srt_l set) t ->
+        forall (B B' : lterm) (t0 : A :: e |- B -> B' : Srt_l prop),
+        P (A :: e) B B' (Srt_l prop) t0 ->
+        P e (Subset_l A B) (Subset_l A' B') (Srt_l set) (tposr_subset t t0)) ->
+       (forall (e : lenv) (A A' : lterm) (s1 : sort)
+          (t : e |- A -> A' : Srt_l s1),
+        P e A A' (Srt_l s1) t ->
+        forall (B B' : lterm) (s2 : sort) (t0 : A :: e |- B -> B' : Srt_l s2),
+        P (A :: e) B B' (Srt_l s2) t0 ->
+        forall (s3 : sort) (s : sum_sort s1 s2 s3),
+        P e (Sum_l A B) (Sum_l A' B') (Srt_l s3) (tposr_sum t t0 s)) ->
+       (forall (e : lenv) (A A' : lterm) (s1 : sort)
+          (t : e |- A -> A' : Srt_l s1),
+        P e A A' (Srt_l s1) t ->
+        forall (B B' : lterm) (s2 : sort) (t0 : A :: e |- B -> B' : Srt_l s2),
+        P (A :: e) B B' (Srt_l s2) t0 ->
+        forall (s3 : sort) (s : sum_sort s1 s2 s3) (t1 t' : lterm)
+          (t2 : e |- t1 -> t' : Sum_l A B),
+        P e t1 t' (Sum_l A B) t2 ->
+        P e (Pi1_l t1) (Pi1_l t') A (tposr_pi1 t t0 s t2)) ->
+       (forall (e : lenv) (A A' : lterm) (s1 : sort)
+          (t : e |- A -> A' : Srt_l s1),
+        P e A A' (Srt_l s1) t ->
+        forall (B B' : lterm) (s2 : sort) (t0 : A :: e |- B -> B' : Srt_l s2),
+        P (A :: e) B B' (Srt_l s2) t0 ->
+        forall (s3 : sort) (s : sum_sort s1 s2 s3) (u u' v v' : lterm)
+          (t1 : e |- Pair_l (Sum_l A B) u v -> Pair_l (Sum_l A' B') u' v'
+                : Sum_l A B),
+        P e (Pair_l (Sum_l A B) u v) (Pair_l (Sum_l A' B') u' v') (Sum_l A B)
+          t1 ->
+        P e (Pi1_l (Pair_l (Sum_l A B) u v)) u A (tposr_pi1_red t t0 s t1)) ->
+       (forall (e : lenv) (A A' : lterm) (s1 : sort)
+          (t : e |- A -> A' : Srt_l s1),
+        P e A A' (Srt_l s1) t ->
+        forall (B B' : lterm) (s2 : sort) (t0 : A :: e |- B -> B' : Srt_l s2),
+        P (A :: e) B B' (Srt_l s2) t0 ->
+        forall (s3 : sort) (s : sum_sort s1 s2 s3) (t1 t' : lterm)
+          (t2 : e |- t1 -> t' : Sum_l A B),
+        P e t1 t' (Sum_l A B) t2 ->
+        P e (Pi2_l t1) (Pi2_l t') (lsubst (Pi1_l t1) B) (tposr_pi2 t t0 s t2)) ->
+       (forall (e : lenv) (A A' : lterm) (s1 : sort)
+          (t : e |- A -> A' : Srt_l s1),
+        P e A A' (Srt_l s1) t ->
+        forall (B B' : lterm) (s2 : sort) (t0 : A :: e |- B -> B' : Srt_l s2),
+        P (A :: e) B B' (Srt_l s2) t0 ->
+        forall (s3 : sort) (s : sum_sort s1 s2 s3) (u u' v v' : lterm)
+          (t1 : e |- Pair_l (Sum_l A B) u v -> Pair_l (Sum_l A' B') u' v'
+                : Sum_l A B),
+        P e (Pair_l (Sum_l A B) u v) (Pair_l (Sum_l A' B') u' v') (Sum_l A B)
+          t1 ->
+        P e (Pi2_l (Pair_l (Sum_l A B) u v)) v (lsubst u B)
+          (tposr_pi2_red t t0 s t1)) ->
+       P0 nil wf_nil ->
+       (forall (G : lenv) (A A' : lterm) (s : sort)
+          (t : G |- A -> A' : Srt_l s),
+        P G A A' (Srt_l s) t -> P0 (A :: G) (wf_cons t)) ->
+       (forall (l : lenv) (l0 l1 l2 : lterm) (t : l |- l0 -> l1 : l2),
+       P l l0 l1 l2 t) /\
+       (forall (l : lenv) (t : tposr_wf l), P0 l t).
+Proof.
+  intros.
+  split.
+  intros.
+  eapply tposr_wf_mutind with (P := P) (P0 := P0) ; auto ; auto.
+  intros.
+  eapply wf_tposr_mutind with (P := P) (P0 := P0) ; auto ; auto.
+Qed.
+
 Inductive tposrp : lenv -> lterm -> lterm -> lterm -> Prop :=
   | tposrp_tposr : forall e X Y Z, e |- X -> Y : Z -> tposrp e X Y Z
   | tposrp_trans : forall e W X Y Z, tposrp e W X Z -> tposrp e X Y Z ->
